\section{Normalisation}

\begin{definition}[Proof Instantiation]
We define a function for replacing all occurences of an open assumption $A^u$ in
a deduction tree $\mathcal{D}$ by a deduction tree $\mathcal{E}$, written as
$\mathcal{D}[A^u/\mathcal{E}]$.

\[
  \mathcal{D}[A^u/\mathcal{E}] =
  \left\{
  \begin{array}{ll}
  \mathcal{E} & \mbox{if } \mathcal{D} = A^u \\[6pt]
  \mathcal{D} & \mbox{if } \mathcal{D} = B^v, v \neq u \\[10pt]
  \mathcal{D} & \mbox{if } \mathcal{D} =
    \AxiomC{$\mathcal{D}'$}
    \noLine
    \UnaryInfC{$C$}
    \RightLabel{$\to$I, $u$}
    \UnaryInfC{$B \to C$}
    \DisplayProof \\[20pt]
  \AxiomC{$\mathcal{D}'[A^u/\mathcal{E}]$}
  \noLine
  \UnaryInfC{$C$}
  \RightLabel{$\to$I, $v$}
  \UnaryInfC{$B \to C$}
  \DisplayProof & \mbox{if } \mathcal{D} =
    \AxiomC{$\mathcal{D}'$}
    \noLine
    \UnaryInfC{$C$}
    \RightLabel{$\to$I, $v$}
    \UnaryInfC{$B \to C$}
    \DisplayProof, v \neq u \\[24pt]
  \AxiomC{$\mathcal{D}'[A^u/\mathcal{E}]$}
  \noLine
  \UnaryInfC{$B \to C$}
  \AxiomC{$\mathcal{D}''[A^u/\mathcal{E}]$}
  \noLine
  \UnaryInfC{$B$}
  \RightLabel{$\to$E}
  \BinaryInfC{$C$}
  \DisplayProof & \mbox{if } \mathcal{D} =
    \AxiomC{$\mathcal{D}'$}
    \noLine
    \UnaryInfC{$B \to C$}
    \AxiomC{$\mathcal{D}''$}
    \noLine
    \UnaryInfC{$B$}
    \RightLabel{$\to$E}
    \BinaryInfC{$C$}
    \DisplayProof
  \end{array}
  \right.
\]
\end{definition}

\begin{definition}[Conversion]
We define a relation $\leadsto \subseteq \npiproofs\times\npiproofs$ that captures the notion of
normalisation steps for \implnpi\ deductions.

\[
  \AxiomC{$[A]^u$}
  \noLine
  \UnaryInfC{$\mathcal{D}$}
  \noLine
  \UnaryInfC{$B$}
  \RightLabel{$\to$I, $u$}
  \UnaryInfC{$A \to B$}
  \AxiomC{$\mathcal{D}_1$}
  \noLine
  \UnaryInfC{$A$}
  \RightLabel{$\to$E}
  \BinaryInfC{$B$}
  \DisplayProof
\ \leadsto\ \mathcal{D}[A^u/\mathcal{D}_1]
\]

\[
  \AxiomC{$[A]^u$}
  \noLine
  \UnaryInfC{$\mathcal{D}$}
  \noLine
  \UnaryInfC{$B$}
  \RightLabel{$\to$I, $u$}
  \UnaryInfC{$A \to B$}
  \DisplayProof
\ \leadsto\ 
  \AxiomC{$[A]^u$}
  \noLine
  \UnaryInfC{$\mathcal{E}$}
  \noLine
  \UnaryInfC{$B$}
  \RightLabel{$\to$I, $u$}
  \UnaryInfC{$A \to B$}
  \DisplayProof
\mbox{if } \mathcal{D} \leadsto \mathcal{E}
\]

\[
  \AxiomC{$\mathcal{D}_1$}
  \noLine
  \UnaryInfC{$A \to B$}
  \AxiomC{$\mathcal{D}_2$}
  \noLine
  \UnaryInfC{$A$}
  \RightLabel{$\to$E}
  \BinaryInfC{$B$}
  \DisplayProof
\ \leadsto\ 
  \AxiomC{$\mathcal{E}_1$}
  \noLine
  \UnaryInfC{$A \to B$}
  \AxiomC{$\mathcal{E}_2$}
  \noLine
  \UnaryInfC{$A$}
  \RightLabel{$\to$E}
  \BinaryInfC{$B$}
  \DisplayProof
\mbox{ if } \mathcal{D}_1 \leadsto \mathcal{E}_1
\mbox{ or } \mathcal{D}_1 \leadsto \mathcal{E}_1
\]
\end{definition}

We now want to show that we can extend the isomorphism for the structures from
\ref{section:bijection} to include the correspondence between conversion in
$\npiproofs$ and $\beta$-reduction in $\stlambdaterms$.

\begin{definition}
\begin{align*}
x^A[M^A/x^A] & := M^A \\
y^B[M^A/x^A] & := y^B \mbox{ for } y \neq x \\
(N_1^{B \to C}N_2^{B})^C[M^A/x^A] & := (N_1^{B \to C}[M^A/x^A]N_2^{B}[M^A/x^A])^C \\
(\lambda x^A.N^B)^{A \to B}[M^A/x^A] & := (\lambda x^A.N^B)^{A \to B} \\
(\lambda y^B.N^C)^{B \to C}[M^A/x^A] & := (\lambda y^B.N^C[M^A/x^A])^{B \to C}
\mbox{ for } y \neq x, y \mbox{ not free in } M^A
\end{align*}
\end{definition}

\begin{proposition}
For $M, M' \in \stlambdaterms$, if $M \betared M'$, then $\chmapanta(M) \leadsto
\chmapanta(M')$.
\end{proposition}

\begin{proof}

As noted in \ref{def:stlambda}, $M \betared M'$ implies that $M = (\lambda
x^A.N^B)^{A \to B}P^A:B$ for some $x, N, P, A, B$ and $M' = N^B[P^A/x^A]$.

To prove our claim, we show that $\chmapanta((\lambda x^A.N^B)^{A \to B}P^A:B) =
\chmapanta(N^B[P^A/x^A])$ by showing that
$\chmapanta(N^B)[\chmapanta(P^A)/\chmapanta(x^A)]) = \chmapanta(N^B[P^A/x^A])$.
The proof is by induction on the construction of $N^B$.

For the base case $N^B \equiv y^B$ there are two possibilities:
\begin{enumerate}[(i)]
  \item $y^B = x^A$, then \\
        $\chmapanta(x^A[P^A/x^A]) = \chmapanta(P^A) =
        A^x[\chmapanta(P^A)/A^x] =
        \chmapanta(x^A)[\chmapanta(P^A)/\chmapanta(x^A)]$
  \item $y^B \not\equiv x^A$, then \\
        $\chmapanta(y^B[P^A/x^A]) = \chmapanta(y^B) = B^y =
        B^y[\chmapanta(P^A)/A^x] =
        \chmapanta(y^B)[\chmapanta(P^A)/\chmapanta(x^A)]$
\end{enumerate}

Assume now that $N_1^{B \to C}, N_2^B$ are two terms such that
\begin{itemize}
\item $\chmapantasub{N_1^{B \to C}}{P^A}{x^A}
      = \subchmapanta{N_1^{B \to C}}{P^A}{x^A}$ and
\item $\chmapantasub{N_2^B}{P^A}{x^A} = \subchmapanta{N_2^B}{P^A}{x^A}$.
\end{itemize}
We treat the case for lambda abstraction with a typed variable $y^D \not\equiv
x^A$. The case where $y^D \equiv x^A$ can be checked by looking at the
definition of subtitution and instantiation and is excluded for brevity. The
case for function application is included the appendix to be referenced if
need be.

\begin{align*}
\lefteqn{\chmapantasub{(\lambda y^D.N_2^B)^{D \to B}}{P^A}{x^A}} \\[10pt]
  &=
  \chmapanta((\lambda y^D.N_2^B[P^A/x^A])^{D \to B})
  \tag{by substitution}\\[10pt]
  % By \chmapanta
  &=
  \implintro{%
    \AxiomC{$\chmapantasub{N_2^B}{P^A}{x^A}$}\noLine\UnaryInfC{$B$}
  }{y}{$D \to B$}
  \DisplayProof \tag{by def. $\chmapanta$}\\[10pt]
  % By i.h.
  &=
  \implintro{%
    \AxiomC{$\subchmapanta{N_2^B}{P^A}{x^A}$}\noLine\UnaryInfC{$B$}
  }{y}{$D \to B$}
  \DisplayProof \tag{by I.H.}\\[10pt]
  % By instantiation
  &=
  \left(
  \implintro{%
    \AxiomC{$\chmapanta(N_2^B)$}\noLine\UnaryInfC{$B$}
  }{y}{$D \to B$}
  \DisplayProof
  \right)[\chmapanta(P^A)/\chmapanta(x^A)] \tag{by instantiation} \\[10pt]
  % By \chmapanta
  &= \subchmapanta{(\lambda y^D.N_2^B)^{D \to B}}{P^A}{x^A} \tag{by def. $\chmapanta$}
\end{align*}

\end{proof}
